CFGraph/HOLCFUtils.thy
@@ -62,6 +62,8 @@ lemma sqsubset_is_subset:"A \<sqsubseteq> B \<longleftrightarrow> A \<subseteq> 
 unfolding below_fun_def and below_bool_def
   by (auto simp:mem_def)
 
+lemmas adm_subset = adm_less[where ?'b = "'a::type set", standard, unfolded sqsubset_is_subset]
+
 lemmas Un_mono_sq =
   subst[OF sqsubset_is_subset[THEN sym], of "\<lambda>x. x",
        OF Un_mono[OF subst[OF sqsubset_is_subset, of "\<lambda>x. x"]
